CertiGC/verif_do_scan.v
@@ -8,7 +8,7 @@ Proof.
   forward_loop (EX index: nat, EX g': LGraph, EX t_info': thread_info,
                 PROP (super_compatible (g', t_info', roots) f_info outlier;
                       forward_condition g' t_info' from to;
-                      thread_info_relation t_info t_info' from;
+                      thread_info_relation t_info t_info';
                       closure_has_index g' to index)
                 LOCAL
                 (temp _s (offset_val (- WORD_SIZE) (vertex_address g' (to, index)));
@@ -21,22 +21,21 @@ Proof.
           PROP (super_compatible (g', t_info', roots) f_info outlier;
                 forward_condition g' t_info' from to;
                 do_scan_relation from to to_index g g';
-                thread_info_relation t_info t_info' from)
+                thread_info_relation t_info t_info')
           LOCAL ()
           SEP (all_string_constants rsh gv; outlier_rep outlier;
                graph_rep g'; thread_info_rep sh t_info' ti)).
-  - Exists to_index g t_info. destruct H as [? [? [? ?]]]. entailer!.
-    apply tir_id.
+  - Exists to_index g t_info. destruct H as [? [? [? ?]]]. entailer!. apply tir_id.
   - Intros index g' t_info'. unfold next_address, thread_info_rep. Intros.
-    unfold heap_struct_rep. destruct H4 as [? [? [? ?]]].
-    destruct H5 as [? [? [? [? ?]]]].
+    unfold heap_struct_rep. destruct H5 as [? [? [? ?]]].
+    destruct H6 as [? [? [? [? ?]]]].
     assert (0 <= Z.of_nat to < 12). {
-      clear -H4 H12. destruct H4 as [_ [_ ?]]. red in H12.
+      clear -H5 H13. destruct H5 as [_ [_ ?]]. red in H13.
       pose proof (spaces_size (ti_heap t_info')).
       rewrite Zlength_correct in H0. rep_omega. } assert (0 < Z.of_nat to) by omega.
-    destruct (gt_gs_compatible _ _ H4 _ H12) as [? [? ?]]. rewrite nth_space_Znth in *.
+    destruct (gt_gs_compatible _ _ H5 _ H13) as [? [? ?]]. rewrite nth_space_Znth in *.
     remember (Znth (Z.of_nat to) (spaces (ti_heap t_info'))) as sp_to.
-    assert (isptr (space_start sp_to)) by (rewrite <- H17; apply start_isptr).
+    assert (isptr (space_start sp_to)) by (rewrite <- H18; apply start_isptr).
     remember ((space_start (heap_head (ti_heap t_info')),
                (Vundef,
                 offset_val (WORD_SIZE * total_space (heap_head (ti_heap t_info')))
@@ -47,21 +46,21 @@ Proof.
       rewrite map_tl, Znth_tl by omega.
       replace (Z.of_nat to - 1 + 1) with (Z.of_nat to) by omega.
       rewrite Znth_map by (rewrite spaces_size; rep_omega). reflexivity. }
-    unfold Inhabitant_pair, Inhabitant_val, Inhabitant in H21.
-    forward; rewrite H21; unfold space_tri. 1: entailer!.
+    unfold Inhabitant_pair, Inhabitant_val, Inhabitant in H22.
+    forward; rewrite H22; unfold space_tri. 1: entailer!.
     unfold vertex_address, vertex_offset. rewrite offset_offset_val. simpl vgeneration.
     simpl vindex.
     replace (WORD_SIZE * (previous_vertices_size g' to index + 1) + - WORD_SIZE) with
         (WORD_SIZE * (previous_vertices_size g' to index))%Z by rep_omega.
-    unfold gen_start at 1. rewrite if_true by assumption. rewrite H17.
+    unfold gen_start at 1. rewrite if_true by assumption. rewrite H18.
     remember (WORD_SIZE * used_space sp_to)%Z as used_offset.
     remember (WORD_SIZE * previous_vertices_size g' to index)%Z as index_offset.
     freeze [0; 1; 3; 4] FR. gather_SEP 1 2. forward_if (gen_has_index g' to index).
     + remember (Znth (Z.of_nat to) (spaces (ti_heap t_info'))) as sp_to.
-      sep_apply (graph_and_heap_rest_data_at_ _ _ _ H12 H4).
+      sep_apply (graph_and_heap_rest_data_at_ _ _ _ H13 H5).
       unfold generation_data_at_.
       assert (gen_start g' to = space_start sp_to) by
-          (subst; unfold gen_start; rewrite if_true; assumption). rewrite H28.
+          (subst; unfold gen_start; rewrite if_true; assumption). rewrite H29.
       rewrite data_at__memory_block. Intros. rewrite sizeof_tarray_int_or_ptr.
       2: unfold gen_size; apply (proj1 (total_space_range (nth_space t_info' to))).
       remember (WORD_SIZE * used_space sp_to)%Z as used_offset.
@@ -70,23 +69,44 @@ Proof.
       simpl. case (peq b b); intros. 2: contradiction. simpl.
       assert (sepalg.nonidentity (nth_sh g' to)). {
         apply readable_nonidentity, writable_readable_share. unfold nth_sh.
-        apply generation_share_writable. } apply andp_right.
-      * change (Vptr b (Ptrofs.add i (Ptrofs.repr index_offset))) with
-            (offset_val index_offset (Vptr b i)).
+        apply generation_share_writable. }
+      assert (forall offset,
+                 0 <= offset <= used_offset ->
+                 memory_block (nth_sh g' to) (WORD_SIZE * gen_size t_info' to)
+                              (Vptr b i) * TT * FRZL FR |--
+        weak_valid_pointer (Vptr b (Ptrofs.add i (Ptrofs.repr offset)))). {
+        intros. change (Vptr b (Ptrofs.add i (Ptrofs.repr offset))) with
+            (offset_val offset (Vptr b i)).
         sep_apply (memory_block_weak_valid_pointer
                      (nth_sh g' to) (WORD_SIZE * gen_size t_info' to)
-                     (Vptr b i) index_offset); auto.
-        3: apply extend_weak_valid_pointer.
-        -- subst. unfold gen_size. split.
-           ++ pose proof (pvs_ge_zero g' to index). rep_omega.
-           ++ apply Zmult_le_compat_l. 2: rep_omega.
-              transitivity (used_space (nth_space t_info' to)).
-              2: apply (proj2 (space_order _)). rewrite nth_space_Znth, <- H19.
-              apply pvs_mono. assumption.
-        -- admit.
-      * admit.
-    + admit.
-    + admit.
+                     (Vptr b i) offset); auto. 3: apply extend_weak_valid_pointer.
+        - subst. unfold gen_size. split. 1: apply (proj1 H32).
+          transitivity (WORD_SIZE * used_space (nth_space t_info' to))%Z.
+          + rewrite nth_space_Znth. apply (proj2 H32).
+          + apply Zmult_le_compat_l. apply (proj2 (space_order _)). rep_omega.
+        - unfold gen_size. clear -H4 H7. destruct H7. unfold gen_size in H0.
+          rewrite <- H0. rewrite nth_space_Znth. rep_omega. }
+      apply andp_right; apply H32.
+      * subst. split. 1: pose proof (pvs_ge_zero g' to index); rep_omega.
+        apply Zmult_le_compat_l. 2: rep_omega. rewrite <- H20.
+        apply pvs_mono. assumption.
+      * split. 2: omega. subst. apply Z.mul_nonneg_nonneg. 1: rep_omega.
+        apply (proj1 (space_order _)).
+    + assert (index_offset < used_offset). {
+        rewrite force_sem_cmp_pp in H23; [|rewrite isptr_offset_val; assumption..].
+        remember (space_start sp_to). destruct v; try contradiction.
+        inv_int i. simpl in H23. rewrite !ptrofs_add_repr in H23.
+        rewrite if_true in H23. 2: reflexivity. unfold typed_true in H23.
+        destruct (Ptrofs.ltu (Ptrofs.repr (ofs + index_offset))
+                             (Ptrofs.repr (ofs + used_offset))) eqn: ?; simpl in H23.
+        2: inversion H23. unfold Ptrofs.ltu in Heqb0.
+        rewrite !Ptrofs.unsigned_repr in Heqb0.
+        - if_tac in Heqb0. 1: omega. inversion Heqb0.
+        - admit.
+        - admit. }
+      forward. entailer!. red. rewrite <- H20 in H24. admit.
+    + forward. thaw FR. unfold thread_info_rep, heap_struct_rep.
+      Exists g' t_info'. unfold forward_condition. entailer!. admit.
     + admit.
   - Intros g' t_info'. forward. Exists g' t_info'. entailer!.
 Abort.
